<?xml version="1.0"?>
<rdf:RDF xmlns="http://semantic-dicom.org/dcm#"
     xml:base="http://semantic-dicom.org/dcm"
     xmlns:owl="http://www.w3.org/2002/07/owl#"
     xmlns:rdf="http://www.w3.org/1999/02/22-rdf-syntax-ns#"
     xmlns:seq="http://semantic-dicom.org/seq#"
     xmlns:xml="http://www.w3.org/XML/1998/namespace"
     xmlns:xsd="http://www.w3.org/2001/XMLSchema#"
     xmlns:rdfs="http://www.w3.org/2000/01/rdf-schema#"
     xmlns:rema="http://semantic-dicom.org/rema#"
     xmlns:dcm-ext="http://semantic-dicom.org/dcm-ext#">

    <owl:Ontology rdf:about="http://semantic-dicom.org/dcm">
        <rdfs:comment rdf:datatype="http://www.w3.org/2001/XMLSchema#string">(c) SOHARD Software GmbH 2015</rdfs:comment>
        <rdfs:comment rdf:datatype="http://www.w3.org/2001/XMLSchema#string">first version with almost complete DICOM standard</rdfs:comment>
        <owl:versionInfo rdf:datatype="http://www.w3.org/2001/XMLSchema#string">0.6 alpha</owl:versionInfo>
    </owl:Ontology>
    

    <!-- 
    ///////////////////////////////////////////////////////////////////////////////////////
    //
    // Annotation properties are given below.
    //
    ///////////////////////////////////////////////////////////////////////////////////////
     -->

    
    <!-- http://semantic-dicom.org/rema#hasKey -->

    <owl:AnnotationProperty rdf:about="http://semantic-dicom.org/rema#hasKey"/>

    <!-- http://www.w3.org/2000/01/rdf-schema#subClassOf -->

    <owl:AnnotationProperty rdf:about="http://www.w3.org/2000/01/rdf-schema#subClassOf"/>
    
    <!-- http://www.w3.org/2002/07/owl#minCardinality -->

    <owl:AnnotationProperty rdf:about="http://www.w3.org/2002/07/owl#minCardinality"/>
    
    <!-- http://www.w3.org/2002/07/owl#minQualifiedCardinality -->

    <owl:AnnotationProperty rdf:about="http://www.w3.org/2002/07/owl#minQualifiedCardinality"/>
    

    <!-- 
    ///////////////////////////////////////////////////////////////////////////////////////
    //
    // Object Properties are given below.
    //
    ///////////////////////////////////////////////////////////////////////////////////////
     -->

    <!-- http://semantic-dicom.org/dcm#WaterEquivalentDiameterCalculationMethodCodeSequence -->
    <owl:ObjectProperty rdf:about="http://semantic-dicom.org/dcm#WaterEquivalentDiameterCalculationMethodCodeSequence">
        <rdfs:comment>
            WaterEquivalentDiameterCalculationMethodCodeSequence is an object property linked to ImageOfCTImage.
        </rdfs:comment>
    </owl:ObjectProperty>
    

    <!-- http://semantic-dicom.org/dcm#containsImage -->
    <owl:ObjectProperty rdf:about="http://semantic-dicom.org/dcm#containsImage">
        <rdfs:subPropertyOf rdf:resource="http://www.w3.org/2002/07/owl#topObjectProperty"/>
        <owl:inverseOf rdf:resource="http://semantic-dicom.org/dcm#isImageOf"/>
        <rdfs:domain rdf:resource="http://semantic-dicom.org/dcm#Series"/>
        <rdfs:range rdf:resource="http://semantic-dicom.org/dcm#Image"/>
        <rdfs:comment>
            containsImage is an object property linking a Series to the Image instances it contains.
        </rdfs:comment>
    </owl:ObjectProperty>
    

    <!-- http://semantic-dicom.org/dcm#containsSeries -->
    <owl:ObjectProperty rdf:about="http://semantic-dicom.org/dcm#containsSeries">
        <rdfs:subPropertyOf rdf:resource="http://www.w3.org/2002/07/owl#topObjectProperty"/>
        <owl:inverseOf rdf:resource="http://semantic-dicom.org/dcm#isSeriesOf"/>
        <rdfs:domain rdf:resource="http://semantic-dicom.org/dcm#Study"/>
        <rdfs:range rdf:resource="http://semantic-dicom.org/dcm#Series"/>
        <rdfs:comment>
            containsSeries is an object property linking a Study to the Series instances it contains.
        </rdfs:comment>
    </owl:ObjectProperty>
    

    <!-- http://semantic-dicom.org/dcm#isImageOf -->
    <owl:ObjectProperty rdf:about="http://semantic-dicom.org/dcm#isImageOf">
        <rdfs:domain rdf:resource="http://semantic-dicom.org/dcm#Image"/>
        <rdfs:range rdf:resource="http://semantic-dicom.org/dcm#Series"/>
        <rdfs:comment>
            isImageOf is an object property linking an Image to the Series it belongs to. It is the inverse of containsImage.
        </rdfs:comment>
    </owl:ObjectProperty>
    

    <!-- http://semantic-dicom.org/dcm#isSeriesOf -->
    <owl:ObjectProperty rdf:about="http://semantic-dicom.org/dcm#isSeriesOf">
        <rdfs:domain rdf:resource="http://semantic-dicom.org/dcm#Series"/>
        <rdfs:range rdf:resource="http://semantic-dicom.org/dcm#Study"/>
        <rdfs:comment>
            isSeriesOf is an object property linking a Series to the Study it belongs to. It is the inverse of containsSeries.
        </rdfs:comment>
    </owl:ObjectProperty>
    

    <!-- http://semantic-dicom.org/dcm#isStudyOf -->
    <owl:ObjectProperty rdf:about="http://semantic-dicom.org/dcm#isStudyOf">
        <rdfs:domain rdf:resource="http://semantic-dicom.org/dcm#Study"/>
        <rdfs:range rdf:resource="http://semantic-dicom.org/dcm#Patient"/>
        <rdfs:comment>
            isStudyOf is an object property linking a Study to the Patient it belongs to. It is the inverse of hasStudy.
        </rdfs:comment>
    </owl:ObjectProperty>
    


    <!-- 
    ///////////////////////////////////////////////////////////////////////////////////////
    //
    // Data properties
    //
    ///////////////////////////////////////////////////////////////////////////////////////
     -->


    <!-- http://semantic-dicom.org/dcm#ImagePositionPatient -->
    <owl:DatatypeProperty rdf:about="http://semantic-dicom.org/dcm#ImagePositionPatient">
        <rdfs:label>Image Position (Patient)</rdfs:label>
        <rdfs:comment>
            ImagePositionPatient is a data property associated with Class Image, representing the x, y, and z coordinates of the upper left hand corner of the image.
        </rdfs:comment>
    </owl:DatatypeProperty>
    

    <!-- http://semantic-dicom.org/dcm#ImagePositionPatient -->

    <owl:DatatypeProperty rdf:about="http://semantic-dicom.org/dcm#ImagePositionPatient">
        <rdfs:range rdf:resource="http://www.w3.org/2001/XMLSchema#string"/>
        <rdfs:domain>
            <owl:Class>
                <owl:unionOf rdf:parseType="Collection">
                    <rdf:Description rdf:about="http://semantic-dicom.org/dcm#Image"/>
                </owl:unionOf>
            </owl:Class>
        </rdfs:domain>
    </owl:DatatypeProperty>
    

    <!-- http://semantic-dicom.org/dcm#ImageOrientationPatient -->
    <owl:DatatypeProperty rdf:about="http://semantic-dicom.org/dcm#ImageOrientationPatient">
        <rdfs:label>Image Orientation (Patient)</rdfs:label>
        <rdfs:comment>
            ImageOrientationPatient is a data property associated with Class Image.
        </rdfs:comment>
    </owl:DatatypeProperty>


    <!-- http://semantic-dicom.org/dcm#ImageOrientationPatient -->

    <owl:DatatypeProperty rdf:about="http://semantic-dicom.org/dcm#ImageOrientationPatient">
        <rdfs:range rdf:resource="http://www.w3.org/2001/XMLSchema#string"/>
        <rdfs:domain>
            <owl:Class>
                <owl:unionOf rdf:parseType="Collection">
                    <rdf:Description rdf:about="http://semantic-dicom.org/dcm#Image"/>
                </owl:unionOf>
            </owl:Class>
        </rdfs:domain>
    </owl:DatatypeProperty>


    <!-- http://semantic-dicom.org/dcm#PatientSize -->

    <owl:DatatypeProperty rdf:about="http://semantic-dicom.org/dcm#PatientSize">
        <rdfs:label>Patient&apos;s Size</rdfs:label>
        <rdfs:comment>
            PatientSize is a data property associated with Study.
        </rdfs:comment>
    </owl:DatatypeProperty>


    <owl:DatatypeProperty rdf:about="http://semantic-dicom.org/dcm#PatientSize">
        <rdfs:label>Patient&apos;s Size</rdfs:label>
        <rdfs:range rdf:resource="&xsd;string"/>
        <rdfs:domain>
            <owl:Class>
                <owl:unionOf rdf:parseType="Collection">
                    <rdf:Description rdf:about="http://semantic-dicom.org/dcm#Study"/>
                </owl:unionOf>
            </owl:Class>
        </rdfs:domain>
    </owl:DatatypeProperty>


    <!-- http://semantic-dicom.org/dcm#PatientSex -->

    <owl:DatatypeProperty rdf:about="http://semantic-dicom.org/dcm#PatientSex">
        <rdfs:label>Patient&apos;s Sex</rdfs:label>
        <rdfs:comment>
            PatientSex is a data property associated with Patient.
        </rdfs:comment>
    </owl:DatatypeProperty>


    <!-- http://semantic-dicom.org/dcm#PatientSex -->

    <owl:DatatypeProperty rdf:about="http://semantic-dicom.org/dcm#PatientSex">
        <rdfs:label>Patient&apos;s Sex</rdfs:label>
        <rdfs:range rdf:resource="&xsd;string"/>
        <rdfs:domain>
            <owl:Class>
                <owl:unionOf rdf:parseType="Collection">
                    <rdf:Description rdf:about="http://semantic-dicom.org/dcm#Patient"/>
                </owl:unionOf>
            </owl:Class>
        </rdfs:domain>
    </owl:DatatypeProperty>


    <!-- http://semantic-dicom.org/dcm#StudyDescription -->

    <owl:DatatypeProperty rdf:about="http://semantic-dicom.org/dcm#StudyDescription">
        <rdfs:label>Study Description</rdfs:label>
        <rdfs:comment>
            StudyDescription is a data property associated with Study.
        </rdfs:comment>
    </owl:DatatypeProperty>


    <!-- http://semantic-dicom.org/dcm#StudyDescription -->

    <owl:DatatypeProperty rdf:about="http://semantic-dicom.org/dcm#StudyDescription">
        <rdfs:label>Study Description</rdfs:label>
        <rdfs:range rdf:resource="&xsd;string"/>
        <rdfs:domain>
            <owl:Class>
                <owl:unionOf rdf:parseType="Collection">
                    <rdf:Description rdf:about="http://semantic-dicom.org/dcm#Study"/>
                </owl:unionOf>
            </owl:Class>
        </rdfs:domain>
    </owl:DatatypeProperty>


    <!-- http://semantic-dicom.org/dcm#AcquisitionDate -->
    <owl:DatatypeProperty rdf:about="http://semantic-dicom.org/dcm#AcquisitionDate">
        <rdfs:label>Acquisition Date</rdfs:label>
        <rdfs:comment>
            AcquisitionDate is a data property associated with Class Image, representing the date the image was acquired.
        </rdfs:comment>
    </owl:DatatypeProperty>
    

    <!-- http://semantic-dicom.org/dcm#AcquisitionNumber -->
    <owl:DatatypeProperty rdf:about="http://semantic-dicom.org/dcm#AcquisitionNumber">
        <rdfs:comment>
            AcquisitionNumber is a data property associated with Class Image, identifying the acquisition process that produced the CT image.
        </rdfs:comment>
    </owl:DatatypeProperty>
    

    <!-- http://semantic-dicom.org/dcm#BitsAllocated -->
    <owl:DatatypeProperty rdf:about="http://semantic-dicom.org/dcm#BitsAllocated">
        <rdfs:comment>
            BitsAllocated is a data property associated with Class Image, representing the number of bits allocated for each pixel sample.
        </rdfs:comment>
    </owl:DatatypeProperty>
    

    <!-- http://semantic-dicom.org/dcm#BitsStored -->
    <owl:DatatypeProperty rdf:about="http://semantic-dicom.org/dcm#BitsStored">
        <rdfs:comment>
            BitsStored is a data property associated with Class Image, representing the number of bits stored for each pixel sample.
        </rdfs:comment>
    </owl:DatatypeProperty>
    

    <!-- http://semantic-dicom.org/dcm#EnergyWeightingFactor -->
    <owl:DatatypeProperty rdf:about="http://semantic-dicom.org/dcm#EnergyWeightingFactor">
        <rdfs:comment>
            EnergyWeightingFactor is a data property associated with Class Image, representing the weighting factor for energy in CT imaging.
        </rdfs:comment>
    </owl:DatatypeProperty>
    

    <!-- http://semantic-dicom.org/dcm#HighBit -->
    <owl:DatatypeProperty rdf:about="http://semantic-dicom.org/dcm#HighBit">
        <rdfs:comment>
            HighBit is a data property associated with Class Image, representing the most significant bit for pixel sample data.
        </rdfs:comment>
    </owl:DatatypeProperty>
    

    <!-- http://semantic-dicom.org/dcm#ImageType -->
    <owl:DatatypeProperty rdf:about="http://semantic-dicom.org/dcm#ImageType">
        <rdfs:comment>
            ImageType is a data property associated with Class Image, that describes the type of the image.
        </rdfs:comment>
    </owl:DatatypeProperty>
    

    <!-- http://semantic-dicom.org/dcm#KVP -->
    <owl:DatatypeProperty rdf:about="http://semantic-dicom.org/dcm#KVP">
        <rdfs:comment>
            KVP is a data property associated with Class Image representing the peak kilo voltage output of the X-Ray generator used.
        </rdfs:comment>
    </owl:DatatypeProperty>
    

    <!-- http://semantic-dicom.org/dcm#Modality -->
    <owl:DatatypeProperty rdf:about="http://semantic-dicom.org/dcm#Modality">
        <rdfs:range rdf:resource="http://www.w3.org/2001/XMLSchema#string"/>
        <rdfs:label>Modality</rdfs:label>
        <rdfs:comment>
            Modality is a data property linked to Series, indicating the type of imaging technique used (for example: CT).
        </rdfs:comment>
    </owl:DatatypeProperty>
    

    <!-- http://semantic-dicom.org/dcm#PatientBirthDate -->
    <owl:DatatypeProperty rdf:about="http://semantic-dicom.org/dcm#PatientBirthDate">
        <rdfs:label>Patient&apos;s Birth Date</rdfs:label>
        <rdfs:comment>
            PatientBirthDate is a data property linked to Patient, representing the birth date of the patient.
        </rdfs:comment>
    </owl:DatatypeProperty>
    

    <!-- http://semantic-dicom.org/dcm#PatientID -->
    <owl:DatatypeProperty rdf:about="http://semantic-dicom.org/dcm#PatientID">
        <rdfs:label>Patient ID</rdfs:label>
        <rdfs:comment>
            PatientID is a data property linked to Patient, representing the primary identifier for the patient.
        </rdfs:comment>
    </owl:DatatypeProperty>
    

    <!-- http://semantic-dicom.org/dcm#PatientName -->
    <owl:DatatypeProperty rdf:about="http://semantic-dicom.org/dcm#PatientName">
        <rdfs:label>Patient&apos;s Name</rdfs:label>
        <rdfs:comment>
            PatientName is a data property linked to Patient, representing the full name of the patient.
        </rdfs:comment>
    </owl:DatatypeProperty>
    

    <!-- http://semantic-dicom.org/dcm#PatientOrientation -->
    <owl:DatatypeProperty rdf:about="http://semantic-dicom.org/dcm#PatientOrientation">
        <rdfs:domain>
            <owl:Class>
                <owl:unionOf rdf:parseType="Collection">
                    <rdf:Description rdf:about="http://semantic-dicom.org/dcm#ImageOfCTImage"/>
                </owl:unionOf>
            </owl:Class>
        </rdfs:domain>
        <rdfs:range rdf:resource="http://www.w3.org/2001/XMLSchema#string"/>
        <rdfs:label>Patient Orientation</rdfs:label>
        <rdfs:comment>
            PatientOrientation is a data property associated with Class Image, describing the patient's orientation relative to the image plane.
        </rdfs:comment>
    </owl:DatatypeProperty>
    

    <!-- http://semantic-dicom.org/dcm#PatientWeight -->
    <owl:DatatypeProperty rdf:about="http://semantic-dicom.org/dcm#PatientWeight">
        <rdfs:domain rdf:resource="http://semantic-dicom.org/dcm#Study"/>
        <rdfs:range rdf:resource="http://www.w3.org/2001/XMLSchema#string"/>
        <rdfs:label>PatientWeight</rdfs:label>
        <rdfs:comment>
            PatientWeight is a data property linked to Study, representing the weight of the patient at the time of the study.
        </rdfs:comment>
    </owl:DatatypeProperty>
    

    <!-- http://semantic-dicom.org/dcm#PatientsAge -->
    <owl:DatatypeProperty rdf:about="http://semantic-dicom.org/dcm#PatientsAge">
        <rdfs:label>Patient&apos;s Age</rdfs:label>
        <rdfs:comment>
            PatientsAge is a data property linked to Study, representing the age of the patient at the time of the study.
        </rdfs:comment>
    </owl:DatatypeProperty>
    

    <!-- http://semantic-dicom.org/dcm#PerformingPhysiciansName -->
    <owl:DatatypeProperty rdf:about="http://semantic-dicom.org/dcm#PerformingPhysiciansName">
        <rdfs:label>Performing Physician&apos;s Name</rdfs:label>
        <rdfs:comment>
            PerformingPhysiciansName is a data property linked to Series, representing the name of the physician performing the series.
        </rdfs:comment>
    </owl:DatatypeProperty>
    

    <!-- http://semantic-dicom.org/dcm#PhotometricInterpretation -->
    <owl:DatatypeProperty rdf:about="http://semantic-dicom.org/dcm#PhotometricInterpretation">
        <rdfs:comment>
            PhotometricInterpretation is a data property that specifies the intended interpretation of the pixel data.
        </rdfs:comment>
    </owl:DatatypeProperty>
    

    <!-- http://semantic-dicom.org/dcm#ReferringPhysicianName -->
    <owl:DatatypeProperty rdf:about="http://semantic-dicom.org/dcm#ReferringPhysicianName">
        <rdfs:label>Referring Physician&apos;s Name</rdfs:label>
        <rdfs:comment>
            ReferringPhysicianName is a data property linked to Study, representing the name of the physician who referred the patient for the study.
        </rdfs:comment>
    </owl:DatatypeProperty>
    

    <!-- http://semantic-dicom.org/dcm#RescaleIntercept -->
    <owl:DatatypeProperty rdf:about="http://semantic-dicom.org/dcm#RescaleIntercept">
        <rdfs:comment>
            RescaleIntercept is a data property associated with Class Image, used for converting stored pixel values to real-world values.
        </rdfs:comment>
    </owl:DatatypeProperty>
    

    <!-- http://semantic-dicom.org/dcm#RescaleSlope -->
    <owl:DatatypeProperty rdf:about="http://semantic-dicom.org/dcm#RescaleSlope">
        <rdfs:comment>
            RescaleSlope is a data property associated with Class Image, used for converting stored pixel values to real-world values.
        </rdfs:comment>
    </owl:DatatypeProperty>
    

    <!-- http://semantic-dicom.org/dcm#RescaleType -->
    <owl:DatatypeProperty rdf:about="http://semantic-dicom.org/dcm#RescaleType">
        <rdfs:comment>
            RescaleType is a data property associated with Class Image, specifying the units of the real world values after rescale operation.
        </rdfs:comment>
    </owl:DatatypeProperty>
    

    <!-- http://semantic-dicom.org/dcm#RetrieveAETitle -->
    <owl:DatatypeProperty rdf:about="http://semantic-dicom.org/dcm#RetrieveAETitle">
        <rdfs:label>Retrieve AE Title</rdfs:label>
        <rdfs:comment>
            RetrieveAETitle is a data property linked to Study, representing the Application Entity title where the instance may be retrieved.
        </rdfs:comment>
    </owl:DatatypeProperty>
    

    <!-- http://semantic-dicom.org/dcm#SOPClassUID -->
    <owl:DatatypeProperty rdf:about="http://semantic-dicom.org/dcm#SOPClassUID">
        <rdfs:subPropertyOf rdf:resource="http://www.w3.org/2002/07/owl#topDataProperty"/>
        <rdfs:label>SOP Class UID</rdfs:label>
        <rdfs:comment>
            SOPClassUID is a data property associated with Class Image, representing the unique identifier for the SOP Class.
        </rdfs:comment>
    </owl:DatatypeProperty>
    

    <!-- http://semantic-dicom.org/dcm#SOPInstanceUID -->
    <owl:DatatypeProperty rdf:about="http://semantic-dicom.org/dcm#SOPInstanceUID">
        <rdfs:label>SOP Instance UID</rdfs:label>
        <rdfs:comment>
            SOPInstanceUID is a data property associated with Class Image, representing the unique identifier for the SOP Instance.
        </rdfs:comment>
    </owl:DatatypeProperty>
    

    <!-- http://semantic-dicom.org/dcm#SamplesPerPixel -->
    <owl:DatatypeProperty rdf:about="http://semantic-dicom.org/dcm#SamplesPerPixel">
        <rdfs:comment>
            SamplesPerPixel is a data property associated with Class Image, representing the number of samples (color channels) per pixel.
        </rdfs:comment>
    </owl:DatatypeProperty>
    

    <!-- http://semantic-dicom.org/dcm#SeriesDate -->
    <owl:DatatypeProperty rdf:about="http://semantic-dicom.org/dcm#SeriesDate">
        <rdfs:range rdf:resource="http://www.w3.org/2001/XMLSchema#string"/>
        <rdfs:label>SeriesDate</rdfs:label>
        <rdfs:comment>
            SeriesDate is a data property linked to Series, representing the date the series was performed.
        </rdfs:comment>
    </owl:DatatypeProperty>
    

    <!-- http://semantic-dicom.org/dcm#StudyDate -->
    <owl:DatatypeProperty rdf:about="http://semantic-dicom.org/dcm#StudyDate">
        <rdfs:label>Study Date</rdfs:label>
        <rdfs:comment>
            StudyDate is a data property linked to Study, representing the date the study was performed.
        </rdfs:comment>
    </owl:DatatypeProperty>
    

    <!-- http://semantic-dicom.org/dcm#StudyID -->
    <owl:DatatypeProperty rdf:about="http://semantic-dicom.org/dcm#StudyID">
        <rdfs:label>Study ID</rdfs:label>
        <rdfs:comment>
            StudyID is a data property linked to Study, representing the identifier for the study assigned by the healthcare provider.
        </rdfs:comment>
    </owl:DatatypeProperty>
    

    <!-- http://semantic-dicom.org/dcm#StudyInstanceUID -->
    <owl:DatatypeProperty rdf:about="http://semantic-dicom.org/dcm#StudyInstanceUID">
        <rdfs:label>Study Instance UID</rdfs:label>
        <rdfs:comment>
            StudyInstanceUID is a data property linked to Study, representing the globally unique identifier for the study.
        </rdfs:comment>
    </owl:DatatypeProperty>
    

    <!-- http://semantic-dicom.org/dcm#StudyTime -->
    <owl:DatatypeProperty rdf:about="http://semantic-dicom.org/dcm#StudyTime">
        <rdfs:label>Study Time</rdfs:label>
        <rdfs:comment>
            StudyTime is a data property linked to Study, representing the time the study was performed.
        </rdfs:comment>
    </owl:DatatypeProperty>
    

    <!-- 
    ///////////////////////////////////////////////////////////////////////////////////////
    //
    // Classes are given below.
    //
    ///////////////////////////////////////////////////////////////////////////////////////
     -->

    

    <!-- http://semantic-dicom.org/dcm#Image -->
    <owl:Class rdf:about="http://semantic-dicom.org/dcm#Image">
        <rdfs:subClassOf rdf:resource="http://semantic-dicom.org/dcm#InformationEntity"/>
        <rdfs:comment>
            Image is a class representing a single medical image, which is part of a Series.
        </rdfs:comment>
    </owl:Class>

    <owl:Class rdf:about="http://semantic-dicom.org/dcm#Image">
        <rdfs:subClassOf>
            <owl:Class>
                <owl:intersectionOf rdf:parseType="Collection">
                    <owl:Restriction>
                        <owl:onProperty rdf:resource="http://semantic-dicom.org/dcm#WaterEquivalentDiameterCalculationMethodCodeSequence"/>
                        <owl:someValuesFrom rdf:resource="http://semantic-dicom.org/dcm#WaterEquivalentDiameterCalculationMethodCodeSequenceType"/>
                    </owl:Restriction>
                    <owl:Restriction>
                        <owl:onProperty rdf:resource="http://semantic-dicom.org/dcm#AcquisitionDate"/>
                        <owl:someValuesFrom rdf:resource="http://www.w3.org/2001/XMLSchema#string"/>
                    </owl:Restriction>
                    <owl:Restriction>
                        <owl:onProperty rdf:resource="http://semantic-dicom.org/dcm#AcquisitionNumber"/>
                        <owl:someValuesFrom rdf:resource="http://www.w3.org/2001/XMLSchema#string"/>
                    </owl:Restriction>
                    <owl:Restriction>
                        <owl:onProperty rdf:resource="http://semantic-dicom.org/dcm#BitsAllocated"/>
                        <owl:someValuesFrom rdf:resource="http://www.w3.org/2001/XMLSchema#string"/>
                    </owl:Restriction>
                    <owl:Restriction>
                        <owl:onProperty rdf:resource="http://semantic-dicom.org/dcm#BitsStored"/>
                        <owl:someValuesFrom rdf:resource="http://www.w3.org/2001/XMLSchema#string"/>
                    </owl:Restriction>
                    <owl:Restriction>
                        <owl:onProperty rdf:resource="http://semantic-dicom.org/dcm#EnergyWeightingFactor"/>
                        <owl:someValuesFrom rdf:resource="http://www.w3.org/2001/XMLSchema#string"/>
                    </owl:Restriction>
                    <owl:Restriction>
                        <owl:onProperty rdf:resource="http://semantic-dicom.org/dcm#HighBit"/>
                        <owl:someValuesFrom rdf:resource="http://www.w3.org/2001/XMLSchema#string"/>
                    </owl:Restriction>
                    <owl:Restriction>
                        <owl:onProperty rdf:resource="http://semantic-dicom.org/dcm#ImageType"/>
                        <owl:someValuesFrom rdf:resource="http://www.w3.org/2001/XMLSchema#string"/>
                    </owl:Restriction>
                    <owl:Restriction>
                        <owl:onProperty rdf:resource="http://semantic-dicom.org/dcm#KVP"/>
                        <owl:someValuesFrom rdf:resource="http://www.w3.org/2001/XMLSchema#string"/>
                    </owl:Restriction>
                    <owl:Restriction>
                        <owl:onProperty rdf:resource="http://semantic-dicom.org/dcm#PatientOrientation"/>
                        <owl:someValuesFrom rdf:resource="http://www.w3.org/2001/XMLSchema#string"/>
                    </owl:Restriction>
                    <owl:Restriction>
                        <owl:onProperty rdf:resource="http://semantic-dicom.org/dcm#PhotometricInterpretation"/>
                        <owl:someValuesFrom rdf:resource="http://www.w3.org/2001/XMLSchema#string"/>
                    </owl:Restriction>
                    <owl:Restriction>
                        <owl:onProperty rdf:resource="http://semantic-dicom.org/dcm#RescaleIntercept"/>
                        <owl:someValuesFrom rdf:resource="http://www.w3.org/2001/XMLSchema#string"/>
                    </owl:Restriction>
                    <owl:Restriction>
                        <owl:onProperty rdf:resource="http://semantic-dicom.org/dcm#RescaleSlope"/>
                        <owl:someValuesFrom rdf:resource="http://www.w3.org/2001/XMLSchema#string"/>
                    </owl:Restriction>
                    <owl:Restriction>
                        <owl:onProperty rdf:resource="http://semantic-dicom.org/dcm#RescaleType"/>
                        <owl:someValuesFrom rdf:resource="http://www.w3.org/2001/XMLSchema#string"/>
                    </owl:Restriction>
                    <owl:Restriction>
                        <owl:onProperty rdf:resource="http://semantic-dicom.org/dcm#SamplesPerPixel"/>
                        <owl:someValuesFrom rdf:resource="http://www.w3.org/2001/XMLSchema#string"/>
                    </owl:Restriction>
                </owl:intersectionOf>
            </owl:Class>
        </rdfs:subClassOf>
    <rdfs:subClassOf>
            <owl:Class>
                <owl:intersectionOf rdf:parseType="Collection">
                    <owl:Restriction>
                        <owl:onProperty rdf:resource="http://semantic-dicom.org/dcm#SOPClassUID"/>
                        <owl:someValuesFrom rdf:resource="http://www.w3.org/2001/XMLSchema#string"/>
                    </owl:Restriction>
                    <owl:Restriction>
                        <owl:onProperty rdf:resource="http://semantic-dicom.org/dcm#SOPInstanceUID"/>
                        <owl:someValuesFrom rdf:resource="http://www.w3.org/2001/XMLSchema#string"/>
                        <rdfs:comment>
                              Each Image has UID which is representing by SOPInstanceUID.
                        </rdfs:comment>
                    </owl:Restriction>
                </owl:intersectionOf>
            </owl:Class>
        </rdfs:subClassOf>
        <rdfs:comment>
            Image is a class representing a single medical image with specific properties and Image is part of a Series.
        </rdfs:comment>
    </owl:Class>



    <!-- http://semantic-dicom.org/dcm#InformationEntity -->
    <owl:Class rdf:about="http://semantic-dicom.org/dcm#InformationEntity">
        <rdfs:comment>
            InformationEntity is the base class for all DICOM information entities in the hierarchy (Patient, Study, Series, Image).
        </rdfs:comment>
    </owl:Class>
    


    <!-- http://semantic-dicom.org/dcm#Patient -->
    <owl:Class rdf:about="http://semantic-dicom.org/dcm#Patient">
        <rdfs:subClassOf rdf:resource="http://semantic-dicom.org/dcm#InformationEntity"/>
        <rdfs:subClassOf>
            <owl:Restriction>
                <owl:onProperty rdf:resource="http://semantic-dicom.org/dcm#PatientBirthDate"/>
                <owl:minCardinality rdf:datatype="http://www.w3.org/2001/XMLSchema#nonNegativeInteger">1</owl:minCardinality>
            </owl:Restriction>
        </rdfs:subClassOf>
        <rdfs:subClassOf>
            <owl:Restriction>
                <owl:onProperty rdf:resource="http://semantic-dicom.org/dcm#PatientID"/>
                <owl:minCardinality rdf:datatype="http://www.w3.org/2001/XMLSchema#nonNegativeInteger">1</owl:minCardinality>
            </owl:Restriction>
        </rdfs:subClassOf>
        <rdfs:subClassOf>
            <owl:Restriction>
                <owl:onProperty rdf:resource="http://semantic-dicom.org/dcm#PatientName"/>
                <owl:minCardinality rdf:datatype="http://www.w3.org/2001/XMLSchema#nonNegativeInteger">1</owl:minCardinality>
            </owl:Restriction>
        </rdfs:subClassOf>
        <owl:disjointWith rdf:resource="http://semantic-dicom.org/dcm#Series"/>
        <owl:disjointWith rdf:resource="http://semantic-dicom.org/dcm#Study"/>
        <rdfs:comment>
            Patient is a class representing a person receiving medical care.
        </rdfs:comment>
    </owl:Class>
    


    <!-- http://semantic-dicom.org/dcm#Series -->
    <owl:Class rdf:about="http://semantic-dicom.org/dcm#Series">
        <rdfs:subClassOf rdf:resource="http://semantic-dicom.org/dcm#InformationEntity"/>
        <rdfs:subClassOf>
            <owl:Restriction>
                <owl:onProperty rdf:resource="http://semantic-dicom.org/dcm#isSeriesOf"/>
                <owl:allValuesFrom rdf:resource="http://semantic-dicom.org/dcm#Study"/>
            </owl:Restriction>
        </rdfs:subClassOf>
        <rdfs:subClassOf>
            <owl:Restriction>
                <owl:onProperty rdf:resource="http://semantic-dicom.org/dcm#isSeriesOf"/>
                <owl:minQualifiedCardinality rdf:datatype="http://www.w3.org/2001/XMLSchema#nonNegativeInteger">1</owl:minQualifiedCardinality>
                <owl:onClass rdf:resource="http://semantic-dicom.org/dcm#Study"/>
            </owl:Restriction>
        </rdfs:subClassOf>
        <rdfs:subClassOf>
            <owl:Restriction>
                <owl:onProperty rdf:resource="http://semantic-dicom.org/dcm#isSeriesOf"/>
                <owl:qualifiedCardinality rdf:datatype="http://www.w3.org/2001/XMLSchema#nonNegativeInteger">1</owl:qualifiedCardinality>
                <owl:onClass rdf:resource="http://semantic-dicom.org/dcm#Study"/>
            </owl:Restriction>
        </rdfs:subClassOf>
        <rdfs:subClassOf>
            <owl:Restriction>
                <owl:onProperty rdf:resource="http://semantic-dicom.org/dcm#Modality"/>
                <owl:someValuesFrom rdf:resource="http://www.w3.org/2001/XMLSchema#string"/>
                <rdfs:comment>
                    Note: A series with modality "CT" represents a CT image acquisition series. 
                </rdfs:comment>
            </owl:Restriction>
        </rdfs:subClassOf>
        <rdfs:subClassOf>
            <owl:Restriction>
                <owl:onProperty rdf:resource="http://semantic-dicom.org/dcm#PerformingPhysiciansName"/>
                <owl:someValuesFrom rdf:resource="http://www.w3.org/2001/XMLSchema#string"/>
                <rdfs:comment>
                    A series has Performing Physicians Name who perform the therapy. 
                </rdfs:comment>
            </owl:Restriction>
        </rdfs:subClassOf>
        <rdfs:subClassOf>
            <owl:Restriction>
                <owl:onProperty rdf:resource="http://semantic-dicom.org/dcm#SeriesDate"/>
                <owl:someValuesFrom rdf:resource="http://www.w3.org/2001/XMLSchema#string"/>
            </owl:Restriction>
        </rdfs:subClassOf>
        <owl:disjointWith rdf:resource="http://semantic-dicom.org/dcm#Study"/>
        <rema:hasKey rdf:resource="http://semantic-dicom.org/dcm#SeriesInstanceUID"/>
        <rdfs:subClassOf>

        </rdfs:subClassOf>
        <rdfs:comment>
            Series is a class representing a collection of related images within a Study, such as a CT scan sequence or MRI sequence.
        </rdfs:comment>
    </owl:Class>
    


    <!-- http://semantic-dicom.org/dcm#Study -->
    <owl:Class rdf:about="http://semantic-dicom.org/dcm#Study">
        <rdfs:subClassOf rdf:resource="http://semantic-dicom.org/dcm#InformationEntity"/>
        <rdfs:subClassOf>
            <owl:Restriction>
                <owl:onProperty rdf:resource="http://semantic-dicom.org/dcm#isStudyOf"/>
                <owl:minQualifiedCardinality rdf:datatype="http://www.w3.org/2001/XMLSchema#nonNegativeInteger">1</owl:minQualifiedCardinality>
                <owl:onClass rdf:resource="http://semantic-dicom.org/dcm#Patient"/>
            </owl:Restriction>
        </rdfs:subClassOf>
        <rdfs:subClassOf>
            <owl:Restriction>
                <owl:onProperty rdf:resource="http://semantic-dicom.org/dcm#PatientWeight"/>
                <owl:someValuesFrom rdf:resource="http://www.w3.org/2001/XMLSchema#string"/>
                <rdfs:comment>
                    Patient Weight is a property linked to Study Class.
                </rdfs:comment>
            </owl:Restriction>
        </rdfs:subClassOf>
        <rdfs:subClassOf>
            <owl:Restriction>
                <owl:onProperty rdf:resource="http://semantic-dicom.org/dcm#PatientsAge"/>
                <owl:someValuesFrom rdf:resource="http://www.w3.org/2001/XMLSchema#string"/>
                <rdfs:comment>
                    Patient Age is a property linked to Study Class.
                </rdfs:comment>
            </owl:Restriction>
        </rdfs:subClassOf>
        <rdfs:subClassOf>
            <owl:Restriction>
                <owl:onProperty rdf:resource="http://semantic-dicom.org/dcm#ReferringPhysicianName"/>
                <owl:minCardinality rdf:datatype="http://www.w3.org/2001/XMLSchema#nonNegativeInteger">1</owl:minCardinality>
            </owl:Restriction>
        </rdfs:subClassOf>
        <rdfs:subClassOf>
            <owl:Restriction>
                <owl:onProperty rdf:resource="http://semantic-dicom.org/dcm#RetrieveAETitle"/>
                <owl:minCardinality rdf:datatype="http://www.w3.org/2001/XMLSchema#nonNegativeInteger">1</owl:minCardinality>
            </owl:Restriction>
        </rdfs:subClassOf>
        <rdfs:subClassOf>
            <owl:Restriction>
                <owl:onProperty rdf:resource="http://semantic-dicom.org/dcm#StudyDate"/>
                <owl:minCardinality rdf:datatype="http://www.w3.org/2001/XMLSchema#nonNegativeInteger">1</owl:minCardinality>
            </owl:Restriction>
        </rdfs:subClassOf>
        <rdfs:subClassOf>
            <owl:Restriction>
                <owl:onProperty rdf:resource="http://semantic-dicom.org/dcm#StudyID"/>
                <owl:minCardinality rdf:datatype="http://www.w3.org/2001/XMLSchema#nonNegativeInteger">1</owl:minCardinality>
            </owl:Restriction>
        </rdfs:subClassOf>
        <rdfs:subClassOf>
            <owl:Restriction>
                <owl:onProperty rdf:resource="http://semantic-dicom.org/dcm#StudyInstanceUID"/>
                <owl:minCardinality rdf:datatype="http://www.w3.org/2001/XMLSchema#nonNegativeInteger">1</owl:minCardinality>
            </owl:Restriction>
        </rdfs:subClassOf>
        <rdfs:subClassOf>
            <owl:Restriction>
                <owl:onProperty rdf:resource="http://semantic-dicom.org/dcm#StudyTime"/>
                <owl:minCardinality rdf:datatype="http://www.w3.org/2001/XMLSchema#nonNegativeInteger">1</owl:minCardinality>
            </owl:Restriction>
        </rdfs:subClassOf>
        <rema:hasKey rdf:resource="http://semantic-dicom.org/dcm#StudyInstanceUID"/>
        <rdfs:comment>
            Study is a class representing a diagnostic study performed on a Patient, containing one or more Series.
        </rdfs:comment>
    </owl:Class>
    


    <!-- http://semantic-dicom.org/dcm#WaterEquivalentDiameterCalculationMethodCodeSequenceType -->
    <owl:Class rdf:about="http://semantic-dicom.org/dcm#WaterEquivalentDiameterCalculationMethodCodeSequenceType">
        <rdfs:comment>
            WaterEquivalentDiameterCalculationMethodCodeSequenceType is a class representing the method used to calculate water equivalent diameter in CT imaging.
        </rdfs:comment>
    </owl:Class>
    <rdf:Description>
        <owl:minCardinality rdf:datatype="http://www.w3.org/2001/XMLSchema#nonNegativeInteger">1</owl:minCardinality>
    </rdf:Description>
    <rdf:Description>
        <owl:minQualifiedCardinality rdf:datatype="http://www.w3.org/2001/XMLSchema#nonNegativeInteger">0</owl:minQualifiedCardinality>
    </rdf:Description>
</rdf:RDF>
